validators

src/lowparse/steel_st_array/LowParse.SteelST.Access.fst
@@ -74,6 +74,42 @@ let parse'
 
 #push-options "--z3rlimit 16"
 
+let peek_strong_with_size
+  (#base: Type)
+  (#k: parser_kind)
+  (#t: Type)
+  (#va: AP.v base byte)
+  (p: parser k t)
+  (a: byte_array base)
+  (sz: SZ.size_t)
+: ST (byte_array base)
+    (AP.arrayptr a va)
+    (fun res -> exists_ (fun vp -> aparse p a vp `star` exists_ (fun vres -> AP.arrayptr res vres `star` pure (
+      let consumed = AP.length (array_of vp) in
+      AP.merge_into (array_of vp) (AP.array_of vres) (AP.array_of va) /\
+      consumed <= AP.length (AP.array_of va) /\
+      AP.contents_of' vres == AP.seq_slice (AP.contents_of' va) consumed (AP.length (AP.array_of va)) /\
+      parse' p (AP.seq_slice (AP.contents_of' va) 0 consumed) == Some (vp.contents, consumed)
+    ))))
+    (k.parser_kind_subkind == Some ParserStrong /\
+      begin match parse' p (AP.contents_of' va) with
+      | None -> False
+      | Some (_, consumed) -> (consumed <: nat) == SZ.size_v sz
+      end
+    )
+    (fun _ -> True)
+=
+  noop ();
+  assert (SZ.size_v sz <= Seq.length (AP.contents_of' va));
+  parse_strong_prefix p (AP.contents_of' va) (AP.seq_slice (AP.contents_of' va) 0 (SZ.size_v sz));
+  let res = AP.split a sz in
+  let _ = gen_elim () in
+  let _ = intro_aparse p a in
+  noop ();
+  return res
+
+#pop-options
+
 let peek_strong
   (#base: Type)
   (#k: parser_kind)
@@ -95,12 +131,61 @@ let peek_strong
       Some? (parse p (AP.contents_of' va)))
     (fun _ -> True)
 =
-  let n = j base _ a in
-  parse_strong_prefix p (AP.contents_of' va) (AP.seq_slice (AP.contents_of' va) 0 (SZ.size_v n));
-  let res = AP.split a n in
-  let _ = gen_elim () in
-  let _ = intro_aparse p a in
+  let sz = j base _ a in
+  let res = peek_strong_with_size p a sz in
   noop ();
   return res
 
-#pop-options
+/// useful for validators, which need to roll back peek after reading some contents
+let unpeek_strong
+  (#opened: _)
+  (#base: Type)
+  (#k: parser_kind)
+  (#t: Type)
+  (#p: parser k t)
+  (#vp: v base k t)
+  (#vres: AP.v base byte)
+  (a: byte_array base)
+  (res: byte_array base)
+: STGhost (AP.v base byte) opened
+    (aparse p a vp `star` AP.arrayptr res vres)
+    (fun va -> AP.arrayptr a va)
+    (AP.adjacent (array_of vp) (AP.array_of vres) /\
+    k.parser_kind_subkind == Some ParserStrong)
+    (fun va ->
+      let consumed = AP.length (array_of vp) in
+      AP.merge_into (array_of vp) (AP.array_of vres) (AP.array_of va) /\
+      consumed <= AP.length (AP.array_of va) /\
+      AP.contents_of' vres == AP.seq_slice (AP.contents_of' va) consumed (AP.length (AP.array_of va)) /\
+      parse' p (AP.seq_slice (AP.contents_of' va) 0 consumed) == Some (vp.contents, consumed) /\
+      parse' p (AP.contents_of' va) == Some (vp.contents, consumed)
+    )
+= let va' = elim_aparse p a in
+  let va = AP.join a res in
+  let consumed = AP.length (array_of vp) in
+  assert (AP.contents_of' vres `Seq.equal` AP.seq_slice (AP.contents_of' va) consumed (AP.length (AP.array_of va)));
+  assert (AP.contents_of' va' `Seq.equal` AP.seq_slice (AP.contents_of' va) 0 consumed);
+  parse_strong_prefix p (AP.contents_of' va') (AP.contents_of' va);
+  noop ();
+  va
+
+let peek_consumes_all
+  (#opened: _)
+  (#base: Type)
+  (#k: parser_kind)
+  (#t: Type)
+  (p: parser k t)
+  (#va: AP.v base byte)
+  (a: byte_array base)
+: STGhost (v base k t) opened
+    (AP.arrayptr a va)
+    (fun vp -> aparse p a vp)
+    (k.parser_kind_subkind == Some ParserConsumesAll /\
+      Some? (parse p (AP.contents_of' va)))
+    (fun vp ->
+      array_of vp == AP.array_of va /\
+      parse' p (AP.contents_of' va) == Some (vp.contents, AP.length (AP.array_of va))
+    )
+=
+  parser_kind_prop_equiv k p;
+  intro_aparse p a
